Optimizations/CanonicalizationSyntax.thy
@@ -521,12 +521,10 @@ proof -
     sorry
 qed
 
-(*
 optimization BinaryFoldConstant: "BinaryExpr op (const e1) (const e2) \<longmapsto> ConstantExpr (bin_eval op e1 e2) when int_and_equal_bits e1 e2 "
    defer apply auto
    apply (simp add: ConstantExpr bin_eval_preserves_validity)
   using nonconstants_gt_one by simp
-*)
 
 optimization AddShiftConstantRight: "((const c) + y) \<longmapsto> y + (const c) when ~(is_ConstantExpr y)"
   defer apply simp
